IsaSAT: split more files

Weidenbach_Book/WB_More_Refinement.thy
@@ -1,8 +1,19 @@
 theory WB_More_Refinement
   imports
-    Refine_Imperative_HOL.IICF
+    "HOL-Library.Cardinality"
+    Refine_Monadic.Refine_Monadic
     Weidenbach_Book_Base.WB_List_More
+    "HOL-Eisbach.Eisbach"
+    Automatic_Refinement.Automatic_Refinement
+    Automatic_Refinement.Relators
+    Refine_Imperative_HOL.Sepref_Misc
+    Refine_Imperative_HOL.Sepref_Intf_Util
 begin
+
+(* taken from IICF*)
+lemma meta_same_imp_rule: "(\<lbrakk>PROP P; PROP P\<rbrakk> \<Longrightarrow> PROP Q) \<equiv> (PROP P \<Longrightarrow> PROP Q)"
+  by rule
+lemma split_prod_bound: "(\<lambda>p. f p) = (\<lambda>(a,b). f (a,b))" by auto
 
 text \<open>This lemma cannot be moved to \<^theory>\<open>Weidenbach_Book_Base.WB_List_More\<close>, because the syntax
  \<^term>\<open>CARD('a)\<close> does not exist there.\<close>
@@ -17,8 +28,6 @@ proof -
 qed
 
 
-no_notation Ref.update ("_ := _" 62)
-
 subsection \<open>Some Tooling for Refinement\<close>
 
 text \<open>
@@ -28,7 +37,7 @@ text \<open>
   appears in the assumptions.
   \<close>
 
-method remove_dummy_vars uses simp =
+method remove_dummy_vars uses simps =
   ((unfold prod.inject)?; (simp only: prod.inject)?; (elim conjE)?;
     hypsubst?; (simp only: triv_forall_equality simps)?)
 
@@ -363,13 +372,6 @@ lemma hn_ctxt_prod_assn_prod:
   unfolding hn_ctxt_def
   by auto
 
-lemma list_assn_map_list_assn: \<open>list_assn g (map f x) xi = list_assn (\<lambda>a c. g (f a) c) x xi\<close>
-  apply (induction x arbitrary: xi)
-  subgoal by auto
-  subgoal for a x xi
-    by (cases xi) auto
-  done
-
 lemma RES_RETURN_RES: \<open>RES \<Phi> \<bind> (\<lambda>T. RETURN (f T)) = RES (f ` \<Phi>)\<close>
   by (simp add: bind_RES_RETURN_eq setcompr_eq_image)
 
@@ -570,14 +572,6 @@ proof -
   finally show ?thesis .
 qed
 
-text \<open>
-  This theorem is useful to debug situation where sepref is not able to synthesize a program (with
-  the ``[[unify\_trace\_failure]]'' to trace what fails in rule rule and the \<^text>\<open>to_hnr\<close> to
-  ensure the theorem has the correct form).
-\<close>
-lemma Pair_hnr: \<open>(uncurry (return oo (\<lambda>a b. Pair a b)), uncurry (RETURN oo (\<lambda>a b. Pair a b))) \<in>
-    A\<^sup>d *\<^sub>a B\<^sup>d \<rightarrow>\<^sub>a prod_assn A B\<close>
-  by sepref_to_hoare sep_auto
 
 lemma fref_weaken_pre_weaken:
   assumes "\<And>x. P x \<longrightarrow> P' x"
@@ -589,13 +583,6 @@ lemma fref_weaken_pre_weaken:
 
 lemma bind_rule_complete_RES: \<open>(M \<bind> f \<le> RES \<Phi>) = (M \<le> SPEC (\<lambda>x. f x \<le> RES \<Phi>))\<close>
   by (auto simp: pw_le_iff refine_pw_simps)
-
-text \<open>This version works only for \<^emph>\<open>pure\<close> refinement relations:\<close>
-lemma the_hnr_keep:
-  \<open>CONSTRAINT is_pure A \<Longrightarrow> (return o the, RETURN o the) \<in> [\<lambda>D. D \<noteq> None]\<^sub>a (option_assn A)\<^sup>k \<rightarrow> A\<close>
-  using pure_option[of A]
-  by sepref_to_hoare
-   (sep_auto simp: option_assn_alt_def is_pure_def split: option.splits)
 
 lemma fref_to_Down:
   \<open>(f, g) \<in> [P]\<^sub>f A \<rightarrow> \<langle>B\<rangle>nres_rel \<Longrightarrow>
@@ -822,69 +809,6 @@ lemma Collect_eq_comp_right:
   \<open>{(x, y). P x y} O {(c, a). a = f c} = {(x, c). \<exists>y. P x y \<and> c = f y} \<close>
   by auto
 
-lemma
-  shows list_mset_assn_add_mset_Nil:
-     \<open>list_mset_assn R (add_mset q Q) [] = false\<close> and
-   list_mset_assn_empty_Cons:
-    \<open>list_mset_assn R {#} (x # xs) = false\<close>
-  unfolding list_mset_assn_def list_mset_rel_def mset_rel_def pure_def p2rel_def
-    rel2p_def rel_mset_def br_def
-  by (sep_auto simp: Collect_eq_comp)+
-
-
-lemma list_mset_assn_add_mset_cons_in:
-  assumes
-    assn: \<open>A \<Turnstile> list_mset_assn R N (ab # list)\<close>
-  shows \<open>\<exists>ab'. (ab, ab') \<in> the_pure R \<and> ab' \<in># N \<and> A \<Turnstile> list_mset_assn R (remove1_mset ab' N) (list)\<close>
-proof -
-  have H: \<open>(\<forall>x x'. (x' = x) = ((x', x) \<in> P')) \<longleftrightarrow> P' = Id\<close> for P'
-    by (auto simp: the_pure_def)
-  have [simp]: \<open>the_pure (\<lambda>a c. \<up> (c = a)) = Id\<close>
-    by (auto simp: the_pure_def H)
-  have [iff]: \<open>(ab # list, y) \<in> list_mset_rel \<longleftrightarrow> y = add_mset ab (mset list)\<close> for y ab list
-    by (auto simp: list_mset_rel_def br_def)
-  obtain N' xs where
-    N_N': \<open>N = mset N'\<close> and
-    \<open>mset xs = add_mset ab (mset list)\<close> and
-    \<open>list_all2 (rel2p (the_pure R)) xs N'\<close>
-    using assn by (cases A) (auto simp: list_mset_assn_def mset_rel_def p2rel_def rel_mset_def
-        rel2p_def)
-  then obtain N'' where
-    \<open>list_all2 (rel2p (the_pure R)) (ab # list) N''\<close> and
-    \<open>mset N'' = mset N'\<close>
-    using list_all2_reorder_left_invariance[of \<open>rel2p (the_pure R)\<close> xs N'
-          \<open>ab # list\<close>, unfolded eq_commute[of \<open>mset (ab # list)\<close>]] by auto
-  then obtain n N''' where
-    n: \<open>add_mset n (mset N''') = mset N''\<close> and
-    \<open>(ab, n) \<in> the_pure R\<close> and
-    \<open>list_all2 (rel2p (the_pure R)) list N'''\<close>
-    by (auto simp: list_all2_Cons1 rel2p_def)
-  moreover have \<open>n \<in> set N''\<close>
-    using n unfolding mset.simps[symmetric] eq_commute[of \<open>add_mset _ _\<close>] apply -
-    by (drule mset_eq_setD) auto
-  ultimately have \<open>(ab, n) \<in> the_pure R\<close> and
-    \<open>n \<in> set N''\<close> and
-    \<open>mset list = mset list\<close> and
-    \<open>mset N''' = remove1_mset n (mset N'')\<close> and
-    \<open>list_all2 (rel2p (the_pure R)) list N'''\<close>
-    by (auto dest: mset_eq_setD simp: eq_commute[of \<open>add_mset _ _\<close>])
-  show ?thesis
-    unfolding list_mset_assn_def mset_rel_def p2rel_def rel_mset_def
-      list.rel_eq list_mset_rel_def
-      br_def N_N'
-    using assn \<open>(ab, n) \<in> the_pure R\<close>  \<open>n \<in> set N''\<close>  \<open>mset N'' = mset N'\<close>
-      \<open>list_all2 (rel2p (the_pure R)) list N'''\<close>
-        \<open>mset N'' = mset N'\<close> \<open>mset N''' = remove1_mset n (mset N'')\<close>
-    by (cases A) (auto simp: list_mset_assn_def mset_rel_def p2rel_def rel_mset_def
-        add_mset_eq_add_mset list.rel_eq
-        intro!: exI[of _ n]
-        dest: mset_eq_setD)
-qed
-
-lemma list_mset_assn_empty_nil: \<open>list_mset_assn R {#} [] = emp\<close>
-  by (auto simp: list_mset_assn_def list_mset_rel_def mset_rel_def
-      br_def p2rel_def rel2p_def Collect_eq_comp rel_mset_def
-      pure_def)
 
 lemma no_fail_spec_le_RETURN_itself: \<open>nofail f \<Longrightarrow> f \<le> SPEC(\<lambda>x. RETURN x \<le> f)\<close>
   by (metis RES_rule nres_order_simps(21) the_RES_inv)
@@ -924,87 +848,15 @@ subsection \<open>More declarations\<close>
 (* TODO: only input notation? *)
 notation prod_rel_syn (infixl "\<times>\<^sub>f" 70)
 
-lemma is_Nil_is_empty[sepref_fr_rules]:
-  \<open>(return o is_Nil, RETURN o Multiset.is_empty) \<in> (list_mset_assn R)\<^sup>k \<rightarrow>\<^sub>a bool_assn\<close>
-  apply sepref_to_hoare
-  apply (rename_tac x xi)
-    apply (case_tac x)
-   by (sep_auto simp: Multiset.is_empty_def list_mset_assn_empty_Cons list_mset_assn_add_mset_Nil
-      split: list.splits)+
 
 lemma diff_add_mset_remove1: \<open>NO_MATCH {#} N \<Longrightarrow> M - add_mset a N = remove1_mset a (M - N)\<close>
   by auto
-
-lemma list_all2_remove:
-  assumes
-    uniq: \<open>IS_RIGHT_UNIQUE (p2rel R)\<close> \<open>IS_LEFT_UNIQUE (p2rel R)\<close> and
-    Ra: \<open>R a aa\<close> and
-    all: \<open>list_all2 R xs ys\<close>
-  shows
-  \<open>\<exists>xs'. mset xs' = remove1_mset a (mset xs) \<and>
-            (\<exists>ys'. mset ys' = remove1_mset aa (mset ys) \<and> list_all2 R xs' ys')\<close>
-  using all
-proof (induction xs ys rule: list_all2_induct)
-  case Nil
-  then show ?case by auto
-next
-  case (Cons x y xs ys) note IH = this(3) and p = this(1, 2)
-
-  have ax: \<open>{#a, x#} = {#x, a#}\<close>
-    by auto
-  have rem1: \<open>remove1_mset a (remove1_mset x M) = remove1_mset x (remove1_mset a M)\<close> for M
-    by (auto simp: ax)
-  have H: \<open>x = a \<longleftrightarrow> y = aa\<close>
-    using uniq Ra p unfolding single_valued_def IS_LEFT_UNIQUE_def p2rel_def by blast
-
-  obtain xs' ys' where
-   \<open>mset xs' = remove1_mset a (mset xs)\<close> and
-   \<open>mset ys' = remove1_mset aa (mset ys)\<close> and
-   \<open>list_all2 R xs' ys'\<close>
-   using IH p by auto
-  then show ?case
-   apply (cases \<open>x \<noteq> a\<close>)
-   subgoal
-     using p
-     by (auto intro!: exI[of _ \<open>x#xs'\<close>] exI[of _ \<open>y#ys'\<close>]
-         simp: diff_add_mset_remove1 rem1 add_mset_remove_trivial_If in_remove1_mset_neq H
-         simp del: diff_diff_add_mset)
-   subgoal
-     using p
-     by (fastforce simp: diff_add_mset_remove1 rem1 add_mset_remove_trivial_If in_remove1_mset_neq
-         remove_1_mset_id_iff_notin H
-         simp del: diff_diff_add_mset)
-   done
-qed
-
-lemma remove1_remove1_mset:
-  assumes uniq: \<open>IS_RIGHT_UNIQUE R\<close> \<open>IS_LEFT_UNIQUE R\<close>
-  shows \<open>(uncurry (RETURN oo remove1), uncurry (RETURN oo remove1_mset)) \<in>
-    R \<times>\<^sub>r (list_mset_rel O \<langle>R\<rangle> mset_rel) \<rightarrow>\<^sub>f
-    \<langle>list_mset_rel O \<langle>R\<rangle> mset_rel\<rangle> nres_rel\<close>
-  using list_all2_remove[of \<open>rel2p R\<close>] assms
-  by (intro frefI nres_relI) (fastforce simp: list_mset_rel_def br_def mset_rel_def p2rel_def
-      rel2p_def[abs_def] rel_mset_def Collect_eq_comp)
-
-lemma
-  Nil_list_mset_rel_iff:
-    \<open>([], aaa) \<in> list_mset_rel \<longleftrightarrow> aaa = {#}\<close> and
-  empty_list_mset_rel_iff:
-    \<open>(a, {#}) \<in> list_mset_rel \<longleftrightarrow> a = []\<close>
-  by (auto simp: list_mset_rel_def br_def)
 
 lemma ex_assn_up_eq2: \<open>(\<exists>\<^sub>Aba. f ba * \<up> (ba = c)) = (f c)\<close>
   by (simp add: ex_assn_def)
 
 lemma ex_assn_pair_split: \<open>(\<exists>\<^sub>Ab. P b) = (\<exists>\<^sub>Aa b. P (a, b))\<close>
   by (subst ex_assn_def, subst (1) ex_assn_def, auto)+
-
-lemma snd_hnr_pure:
-   \<open>CONSTRAINT is_pure B \<Longrightarrow> (return \<circ> snd, RETURN \<circ> snd) \<in> A\<^sup>d *\<^sub>a B\<^sup>k \<rightarrow>\<^sub>a B\<close>
-  apply sepref_to_hoare
-  apply sep_auto
-  by (metis SLN_def SLN_left assn_times_comm ent_pure_pre_iff_sng ent_refl ent_star_mono
-      ent_true is_pure_assn_def is_pure_iff_pure_assn)
 
 
 subsection \<open>List relation\<close>
@@ -1055,68 +907,13 @@ lemma list_rel_in_find_correspondanceE:
   using assms[unfolded in_set_conv_decomp] by (auto simp: list_rel_append1
       elim!: list_relE3)
 
-definition list_rel_mset_rel where list_rel_mset_rel_internal:
-\<open>list_rel_mset_rel \<equiv> \<lambda>R. \<langle>R\<rangle>list_rel O list_mset_rel\<close>
-
-lemma list_rel_mset_rel_def[refine_rel_defs]:
-  \<open>\<langle>R\<rangle>list_rel_mset_rel = \<langle>R\<rangle>list_rel O list_mset_rel\<close>
-  unfolding relAPP_def list_rel_mset_rel_internal ..
-
-lemma list_mset_assn_pure_conv:
-  \<open>list_mset_assn (pure R) = pure (\<langle>R\<rangle>list_rel_mset_rel)\<close>
-  apply (intro ext)
-  using list_all2_reorder_left_invariance
-  by (fastforce
-    simp: list_rel_mset_rel_def list_mset_assn_def
-      mset_rel_def rel2p_def[abs_def] rel_mset_def p2rel_def
-      list_mset_rel_def[abs_def] Collect_eq_comp br_def
-      list_rel_def Collect_eq_comp_right
-    intro!: arg_cong[of _ _ \<open>\<lambda>b. pure b _ _\<close>])
-
-lemma list_assn_list_mset_rel_eq_list_mset_assn:
-  assumes p: \<open>is_pure R\<close>
-  shows \<open>hr_comp (list_assn R) list_mset_rel = list_mset_assn R\<close>
-proof -
-  define R' where \<open>R' = the_pure R\<close>
-  then have R: \<open>R = pure R'\<close>
-    using p by auto
-  show ?thesis
-    apply (auto simp: list_mset_assn_def
-        list_assn_pure_conv
-        relcomp.simps hr_comp_pure mset_rel_def br_def
-        p2rel_def rel2p_def[abs_def] rel_mset_def R list_mset_rel_def list_rel_def)
-      using list_all2_reorder_left_invariance by fastforce
-  qed
-
-lemma list_rel_mset_rel_imp_same_length: \<open>(a, b) \<in> \<langle>R\<rangle>list_rel_mset_rel \<Longrightarrow> length a = size b\<close>
-  by (auto simp: list_rel_mset_rel_def list_mset_rel_def br_def
-      dest: list_rel_imp_same_length)
 
 
 subsection \<open>More Functions, Relations, and Theorems\<close>
 
-lemma id_ref: \<open>(return o id, RETURN o id) \<in> R\<^sup>d \<rightarrow>\<^sub>a R\<close>
-  by sepref_to_hoare sep_auto
-
 definition emptied_list :: \<open>'a list \<Rightarrow> 'a list\<close> where
   \<open>emptied_list l = []\<close>
 
-text \<open>This functions deletes all elements of a resizable array, without resizing it.\<close>
-definition emptied_arl :: \<open>'a array_list \<Rightarrow> 'a array_list\<close> where
-\<open>emptied_arl = (\<lambda>(a, n). (a, 0))\<close>
-
-lemma emptied_arl_refine[sepref_fr_rules]:
-  \<open>(return o emptied_arl, RETURN o emptied_list) \<in> (arl_assn R)\<^sup>d \<rightarrow>\<^sub>a arl_assn R\<close>
-  unfolding emptied_arl_def emptied_list_def
-  by sepref_to_hoare (sep_auto simp: arl_assn_def hr_comp_def is_array_list_def)
-
-lemma bool_assn_alt_def: \<open>bool_assn a b = \<up> (a = b)\<close>
-  unfolding pure_def by auto
-
-lemma nempty_list_mset_rel_iff: \<open>M \<noteq> {#} \<Longrightarrow>
-  (xs, M) \<in> list_mset_rel \<longleftrightarrow> (xs \<noteq> [] \<and> hd xs \<in># M \<and>
-         (tl xs, remove1_mset (hd xs) M) \<in> list_mset_rel)\<close>
-  by (cases xs) (auto simp: list_mset_rel_def br_def dest!: multi_member_split)
 
 lemma Down_id_eq: "\<Down> Id a = a"
   by auto
@@ -1216,12 +1013,6 @@ definition virtual_copy where
 definition virtual_copy_rel where
   \<open>virtual_copy_rel = {(c, b). c = ()}\<close>
 
-abbreviation ghost_assn where
-  \<open>ghost_assn \<equiv> hr_comp unit_assn virtual_copy_rel\<close>
-
-lemma [sepref_fr_rules]:
- \<open>(return o (\<lambda>_. ()), RETURN o virtual_copy) \<in> R\<^sup>k \<rightarrow>\<^sub>a ghost_assn\<close>
- by sepref_to_hoare (sep_auto simp: virtual_copy_rel_def)
 
 lemma bind_cong_nres: \<open>(\<And>x. g x = g' x) \<Longrightarrow> (do {a \<leftarrow> f :: 'a nres;  g a}) = (do {a \<leftarrow> f :: 'a nres;  g' a})\<close>
   by auto
@@ -1388,21 +1179,6 @@ lemma RES_RES13_RETURN_RES: \<open>do {
       vdom avdom lcount)\<close>
   by (force simp:  pw_eq_iff refine_pw_simps uncurry_def)
 
-lemma id_mset_list_assn_list_mset_assn:
-  assumes \<open>CONSTRAINT is_pure R\<close>
-  shows \<open>(return o id, RETURN o mset) \<in> (list_assn R)\<^sup>d \<rightarrow>\<^sub>a list_mset_assn R\<close>
-proof -
-  obtain R' where R: \<open>R = pure R'\<close>
-    using assms is_pure_conv unfolding CONSTRAINT_def by blast
-  then have R': \<open>the_pure R = R'\<close>
-    unfolding R by auto
-  show ?thesis
-    apply (subst R)
-    apply (subst list_assn_pure_conv)
-    apply sepref_to_hoare
-    by (sep_auto simp: list_mset_assn_def R' pure_def list_mset_rel_def mset_rel_def
-       p2rel_def rel2p_def[abs_def] rel_mset_def br_def Collect_eq_comp list_rel_def)
-qed
 
 lemma RES_SPEC_conv: \<open>RES P = SPEC (\<lambda>v. v \<in> P)\<close>
   by auto
@@ -1412,206 +1188,6 @@ lemma add_invar_refineI_P: \<open>A \<le> \<Down> {(x,y). R x y} B \<Longrightar
   by auto
 
 
-subsection \<open>Sorting\<close>
-
-text \<open>Remark that we do not \<^emph>\<open>prove\<close> that the sorting in correct, since we do not care about the
- correctness, only the fact that it is reordered. (Based on wikipedia's algorithm.)
-Typically \<^term>\<open>R\<close> would be \<^term>\<open>(<)\<close>\<close>
-definition insert_sort_inner :: \<open>('b \<Rightarrow> 'b \<Rightarrow> bool) \<Rightarrow> ('a list \<Rightarrow> nat \<Rightarrow> 'b) \<Rightarrow> 'a list \<Rightarrow>  nat \<Rightarrow> 'a list nres\<close> where
-  \<open>insert_sort_inner R f xs i = do {
-     (j, ys) \<leftarrow> WHILE\<^sub>T\<^bsup>\<lambda>(j, ys). j \<ge> 0 \<and> mset xs = mset ys \<and> j < length ys\<^esup>
-         (\<lambda>(j, ys). j > 0 \<and> R (f ys j) (f ys (j - 1)))
-         (\<lambda>(j, ys). do {
-             ASSERT(j < length ys);
-             ASSERT(j > 0);
-             ASSERT(j-1 < length ys);
-             let xs = swap ys j (j - 1);
-             RETURN (j-1, xs)
-           }
-         )
-        (i, xs);
-     RETURN ys
-  }\<close>
-
-
-(* A check: *)
-lemma \<open>RETURN [Suc 0, 2, 0] = insert_sort_inner (<) (\<lambda>remove n. remove ! n) [2::nat, 1, 0] 1\<close>
-  by (simp add: WHILEIT_unfold insert_sort_inner_def swap_def)
-
-definition reorder_remove :: \<open>'b \<Rightarrow> 'a list \<Rightarrow> 'a list nres\<close> where
-\<open>reorder_remove _ removed = SPEC (\<lambda>removed'. mset removed' = mset removed)\<close>
-
-definition insert_sort :: \<open>('b \<Rightarrow> 'b \<Rightarrow> bool) \<Rightarrow> ('a list \<Rightarrow> nat \<Rightarrow> 'b) \<Rightarrow> 'a list \<Rightarrow> 'a list nres\<close> where
-  \<open>insert_sort R f xs = do {
-     (i, ys) \<leftarrow> WHILE\<^sub>T\<^bsup>\<lambda>(i, ys). (ys = [] \<or> i \<le> length ys) \<and> mset xs = mset ys\<^esup>
-        (\<lambda>(i, ys). i < length ys)
-        (\<lambda>(i, ys). do {
-            ASSERT(i < length ys);
-            ys \<leftarrow> insert_sort_inner R f ys i;
-            RETURN (i+1, ys)
-          })
-        (1, xs);
-     RETURN ys
-  }\<close>
-
-lemma insert_sort_inner:
-   \<open>(uncurry (insert_sort_inner R f), uncurry (\<lambda>m m'. reorder_remove m' m)) \<in>
-      [\<lambda>(xs, i). i < length xs]\<^sub>f \<langle>Id:: ('a \<times> 'a) set\<rangle>list_rel \<times>\<^sub>r nat_rel \<rightarrow> \<langle>Id\<rangle> nres_rel\<close>
-  unfolding insert_sort_inner_def uncurry_def reorder_remove_def
-  apply (intro frefI nres_relI)
-  apply clarify
-  apply (refine_vcg WHILEIT_rule[where R = \<open>measure (\<lambda>(i, _). i)\<close>])
-  subgoal by auto
-  subgoal by auto
-  subgoal by auto
-  subgoal by auto
-  subgoal by (auto dest: mset_eq_length)
-  subgoal by auto
-  subgoal by auto
-  subgoal by auto
-  subgoal by auto
-  subgoal by auto
-  subgoal by auto
-  subgoal by auto
-  done
-
-lemma insert_sort_reorder_remove:
-  \<open>(insert_sort R f, reorder_remove vm) \<in> \<langle>Id\<rangle>list_rel \<rightarrow>\<^sub>f \<langle>Id\<rangle> nres_rel\<close>
-proof -
-  have H: \<open>ba < length aa \<Longrightarrow> insert_sort_inner R f aa ba \<le> SPEC (\<lambda>m'. mset m' = mset aa)\<close>
-    for ba aa
-    using insert_sort_inner[unfolded fref_def nres_rel_def reorder_remove_def, simplified]
-    by fast
-  show ?thesis
-    unfolding insert_sort_def reorder_remove_def
-    apply (intro frefI nres_relI)
-    apply (refine_vcg WHILEIT_rule[where R = \<open>measure (\<lambda>(i, ys). length ys - i)\<close>] H)
-    subgoal by auto
-    subgoal by auto
-    subgoal by auto
-    subgoal by auto
-    subgoal by (auto dest: mset_eq_length)
-    subgoal by auto
-    subgoal by (auto dest!: mset_eq_length)
-    subgoal by auto
-    done
-qed
-
-definition arl_replicate where
- "arl_replicate init_cap x \<equiv> do {
-    let n = max init_cap minimum_capacity;
-    a \<leftarrow> Array.new n x;
-    return (a,init_cap)
-  }"
-
-definition \<open>op_arl_replicate = op_list_replicate\<close>
-lemma arl_fold_custom_replicate:
-  \<open>replicate = op_arl_replicate\<close>
-  unfolding op_arl_replicate_def op_list_replicate_def ..
-
-lemma list_replicate_arl_hnr[sepref_fr_rules]:
-  assumes p: \<open>CONSTRAINT is_pure R\<close>
-  shows \<open>(uncurry arl_replicate, uncurry (RETURN oo op_arl_replicate)) \<in> nat_assn\<^sup>k *\<^sub>a R\<^sup>k \<rightarrow>\<^sub>a arl_assn R\<close>
-proof -
-  obtain R' where
-     R'[symmetric]: \<open>R' = the_pure R\<close> and
-     R_R': \<open>R = pure R'\<close>
-    using assms by fastforce
-  have [simp]: \<open>pure R' b bi = \<up>((bi, b) \<in> R')\<close> for b bi
-    by (auto simp: pure_def)
-  have [simp]: \<open>min a (max a 16) = a\<close> for a :: nat
-    by auto
-  show ?thesis
-    using assms unfolding op_arl_replicate_def
-    by sepref_to_hoare
-      (sep_auto simp: arl_replicate_def arl_assn_def hr_comp_def R' R_R' list_rel_def
-        is_array_list_def minimum_capacity_def
-        intro!: list_all2_replicate)
-qed
-
-lemma option_bool_assn_direct_eq_hnr:
-  \<open>(uncurry (return oo (=)), uncurry (RETURN oo (=))) \<in>
-    (option_assn bool_assn)\<^sup>k *\<^sub>a (option_assn bool_assn)\<^sup>k \<rightarrow>\<^sub>a bool_assn\<close>
-  by sepref_to_hoare (sep_auto simp: option_assn_alt_def split:option.splits)
-
-text \<open>This function does not change the size of the underlying array.\<close>
-definition take1 where
-  \<open>take1 xs = take 1 xs\<close>
-
-lemma take1_hnr[sepref_fr_rules]:
-  \<open>(return o (\<lambda>(a, _). (a, 1::nat)), RETURN o take1) \<in> [\<lambda>xs. xs \<noteq> []]\<^sub>a (arl_assn R)\<^sup>d \<rightarrow> arl_assn R\<close>
-  apply sepref_to_hoare
-  apply (sep_auto simp: arl_assn_def hr_comp_def take1_def list_rel_def
-      is_array_list_def)
-  apply (case_tac b; case_tac x; case_tac l')
-   apply (auto)
-  done
-
-text \<open>The following two abbreviation are variants from \<^term>\<open>uncurry4\<close> and
-   \<^term>\<open>uncurry6\<close>. The problem is that \<^term>\<open>uncurry2 (uncurry2 f)\<close> and
-   \<^term>\<open>uncurry (uncurry3 f)\<close> are the same term, but only the latter is folded
-   to \<^term>\<open>uncurry4\<close>.\<close>
-abbreviation uncurry4' where
-  "uncurry4' f \<equiv> uncurry2 (uncurry2 f)"
-
-abbreviation uncurry6' where
-  "uncurry6' f \<equiv> uncurry2 (uncurry4' f)"
-
-
-definition find_in_list_between :: \<open>('a \<Rightarrow> bool) \<Rightarrow> nat \<Rightarrow> nat \<Rightarrow> 'a list \<Rightarrow> nat option nres\<close> where
-  \<open>find_in_list_between P a b C = do {
-      (x, _) \<leftarrow> WHILE\<^sub>T\<^bsup>\<lambda>(found, i). i \<ge> a \<and> i \<le> length C \<and> i \<le> b \<and> (\<forall>j\<in>{a..<i}. \<not>P (C!j)) \<and>
-        (\<forall>j. found = Some j \<longrightarrow> (i = j \<and> P (C ! j) \<and> j < b \<and> j \<ge> a))\<^esup>
-        (\<lambda>(found, i). found = None \<and> i < b)
-        (\<lambda>(_, i). do {
-          ASSERT(i < length C);
-          if P (C!i) then RETURN (Some i, i) else RETURN (None, i+1)
-        })
-        (None, a);
-      RETURN x
-  }\<close>
-
-lemma find_in_list_between_spec:
-  assumes \<open>a \<le> length C\<close> and \<open>b \<le> length C\<close> and \<open>a \<le> b\<close>
-  shows
-    \<open>find_in_list_between P a b C \<le> SPEC(\<lambda>i.
-       (i \<noteq> None \<longrightarrow>  P (C ! the i) \<and> the i \<ge> a \<and> the i < b) \<and>
-       (i = None \<longrightarrow> (\<forall>j. j \<ge> a \<longrightarrow> j < b \<longrightarrow> \<not>P (C!j))))\<close>
-  unfolding find_in_list_between_def
-  apply (refine_vcg WHILEIT_rule[where R = \<open>measure (\<lambda>(f, i). Suc (length C) - (i + (if f = None then 0 else 1)))\<close>])
-  subgoal by auto
-  subgoal by auto
-  subgoal using assms by auto
-  subgoal using assms by auto
-  subgoal by auto
-  subgoal by auto
-  subgoal by auto
-  subgoal by auto
-  subgoal by auto
-  subgoal using assms by auto
-  subgoal by auto
-  subgoal by auto
-  subgoal by auto
-  subgoal by auto
-  subgoal by auto
-  subgoal by auto
-  subgoal by auto
-  subgoal by auto
-  subgoal by auto
-  subgoal by auto
-  subgoal by auto
-  subgoal by auto
-  subgoal by (auto simp: less_Suc_eq)
-  subgoal by auto
-  subgoal by auto
-  subgoal by auto
-  subgoal by auto
-  subgoal by auto
-  subgoal by auto
-  subgoal by auto
-  subgoal by auto
-  subgoal by auto
-  done
 
 lemma same_in_Id_option_rel:
   \<open>x = x' \<Longrightarrow> (x, x') \<in> \<langle>Id\<rangle>option_rel\<close>
