Weidenbach_Book/IsaSAT_Setup_SML.thy
@@ -1,0 +1,5 @@
+theory IsaSAT_Setup_SML
+imports IsaSAT_Setup
+begin
+
+end
