Weidenbach_Book/WB_More_IICF_SML.thy
@@ -1,0 +1,451 @@
+theory WB_More_IICF_SML
+imports Refine_Imperative_HOL.IICF WB_More_Refinement
+begin
+
+lemma
+  shows list_mset_assn_add_mset_Nil:
+     \<open>list_mset_assn R (add_mset q Q) [] = false\<close> and
+   list_mset_assn_empty_Cons:
+    \<open>list_mset_assn R {#} (x # xs) = false\<close>
+  unfolding list_mset_assn_def list_mset_rel_def mset_rel_def pure_def p2rel_def
+    rel2p_def rel_mset_def br_def
+  by (sep_auto simp: Collect_eq_comp)+
+
+
+lemma list_mset_assn_add_mset_cons_in:
+  assumes
+    assn: \<open>A \<Turnstile> list_mset_assn R N (ab # list)\<close>
+  shows \<open>\<exists>ab'. (ab, ab') \<in> the_pure R \<and> ab' \<in># N \<and> A \<Turnstile> list_mset_assn R (remove1_mset ab' N) (list)\<close>
+proof -
+  have H: \<open>(\<forall>x x'. (x' = x) = ((x', x) \<in> P')) \<longleftrightarrow> P' = Id\<close> for P'
+    by (auto simp: the_pure_def)
+  have [simp]: \<open>the_pure (\<lambda>a c. \<up> (c = a)) = Id\<close>
+    by (auto simp: the_pure_def H)
+  have [iff]: \<open>(ab # list, y) \<in> list_mset_rel \<longleftrightarrow> y = add_mset ab (mset list)\<close> for y ab list
+    by (auto simp: list_mset_rel_def br_def)
+  obtain N' xs where
+    N_N': \<open>N = mset N'\<close> and
+    \<open>mset xs = add_mset ab (mset list)\<close> and
+    \<open>list_all2 (rel2p (the_pure R)) xs N'\<close>
+    using assn by (cases A) (auto simp: list_mset_assn_def mset_rel_def p2rel_def rel_mset_def
+        rel2p_def)
+  then obtain N'' where
+    \<open>list_all2 (rel2p (the_pure R)) (ab # list) N''\<close> and
+    \<open>mset N'' = mset N'\<close>
+    using list_all2_reorder_left_invariance[of \<open>rel2p (the_pure R)\<close> xs N'
+          \<open>ab # list\<close>, unfolded eq_commute[of \<open>mset (ab # list)\<close>]] by auto
+  then obtain n N''' where
+    n: \<open>add_mset n (mset N''') = mset N''\<close> and
+    \<open>(ab, n) \<in> the_pure R\<close> and
+    \<open>list_all2 (rel2p (the_pure R)) list N'''\<close>
+    by (auto simp: list_all2_Cons1 rel2p_def)
+  moreover have \<open>n \<in> set N''\<close>
+    using n unfolding mset.simps[symmetric] eq_commute[of \<open>add_mset _ _\<close>] apply -
+    by (drule mset_eq_setD) auto
+  ultimately have \<open>(ab, n) \<in> the_pure R\<close> and
+    \<open>n \<in> set N''\<close> and
+    \<open>mset list = mset list\<close> and
+    \<open>mset N''' = remove1_mset n (mset N'')\<close> and
+    \<open>list_all2 (rel2p (the_pure R)) list N'''\<close>
+    by (auto dest: mset_eq_setD simp: eq_commute[of \<open>add_mset _ _\<close>])
+  show ?thesis
+    unfolding list_mset_assn_def mset_rel_def p2rel_def rel_mset_def
+      list.rel_eq list_mset_rel_def
+      br_def N_N'
+    using assn \<open>(ab, n) \<in> the_pure R\<close>  \<open>n \<in> set N''\<close>  \<open>mset N'' = mset N'\<close>
+      \<open>list_all2 (rel2p (the_pure R)) list N'''\<close>
+        \<open>mset N'' = mset N'\<close> \<open>mset N''' = remove1_mset n (mset N'')\<close>
+    by (cases A) (auto simp: list_mset_assn_def mset_rel_def p2rel_def rel_mset_def
+        add_mset_eq_add_mset list.rel_eq
+        intro!: exI[of _ n]
+        dest: mset_eq_setD)
+qed
+
+lemma list_mset_assn_empty_nil: \<open>list_mset_assn R {#} [] = emp\<close>
+  by (auto simp: list_mset_assn_def list_mset_rel_def mset_rel_def
+      br_def p2rel_def rel2p_def Collect_eq_comp rel_mset_def
+      pure_def)
+
+lemma is_Nil_is_empty[sepref_fr_rules]:
+  \<open>(return o is_Nil, RETURN o Multiset.is_empty) \<in> (list_mset_assn R)\<^sup>k \<rightarrow>\<^sub>a bool_assn\<close>
+  apply sepref_to_hoare
+  apply (rename_tac x xi)
+    apply (case_tac x)
+   by (sep_auto simp: Multiset.is_empty_def list_mset_assn_empty_Cons list_mset_assn_add_mset_Nil
+      split: list.splits)+
+
+
+lemma list_all2_remove:
+  assumes
+    uniq: \<open>IS_RIGHT_UNIQUE (p2rel R)\<close> \<open>IS_LEFT_UNIQUE (p2rel R)\<close> and
+    Ra: \<open>R a aa\<close> and
+    all: \<open>list_all2 R xs ys\<close>
+  shows
+  \<open>\<exists>xs'. mset xs' = remove1_mset a (mset xs) \<and>
+            (\<exists>ys'. mset ys' = remove1_mset aa (mset ys) \<and> list_all2 R xs' ys')\<close>
+  using all
+proof (induction xs ys rule: list_all2_induct)
+  case Nil
+  then show ?case by auto
+next
+  case (Cons x y xs ys) note IH = this(3) and p = this(1, 2)
+
+  have ax: \<open>{#a, x#} = {#x, a#}\<close>
+    by auto
+  have rem1: \<open>remove1_mset a (remove1_mset x M) = remove1_mset x (remove1_mset a M)\<close> for M
+    by (auto simp: ax)
+  have H: \<open>x = a \<longleftrightarrow> y = aa\<close>
+    using uniq Ra p unfolding single_valued_def IS_LEFT_UNIQUE_def p2rel_def by blast
+
+  obtain xs' ys' where
+   \<open>mset xs' = remove1_mset a (mset xs)\<close> and
+   \<open>mset ys' = remove1_mset aa (mset ys)\<close> and
+   \<open>list_all2 R xs' ys'\<close>
+   using IH p by auto
+  then show ?case
+   apply (cases \<open>x \<noteq> a\<close>)
+   subgoal
+     using p
+     by (auto intro!: exI[of _ \<open>x#xs'\<close>] exI[of _ \<open>y#ys'\<close>]
+         simp: diff_add_mset_remove1 rem1 add_mset_remove_trivial_If in_remove1_mset_neq H
+         simp del: diff_diff_add_mset)
+   subgoal
+     using p
+     by (fastforce simp: diff_add_mset_remove1 rem1 add_mset_remove_trivial_If in_remove1_mset_neq
+         remove_1_mset_id_iff_notin H
+         simp del: diff_diff_add_mset)
+   done
+qed
+
+lemma remove1_remove1_mset:
+  assumes uniq: \<open>IS_RIGHT_UNIQUE R\<close> \<open>IS_LEFT_UNIQUE R\<close>
+  shows \<open>(uncurry (RETURN oo remove1), uncurry (RETURN oo remove1_mset)) \<in>
+    R \<times>\<^sub>r (list_mset_rel O \<langle>R\<rangle> mset_rel) \<rightarrow>\<^sub>f
+    \<langle>list_mset_rel O \<langle>R\<rangle> mset_rel\<rangle> nres_rel\<close>
+  using list_all2_remove[of \<open>rel2p R\<close>] assms
+  by (intro frefI nres_relI) (fastforce simp: list_mset_rel_def br_def mset_rel_def p2rel_def
+      rel2p_def[abs_def] rel_mset_def Collect_eq_comp)
+
+lemma
+  Nil_list_mset_rel_iff:
+    \<open>([], aaa) \<in> list_mset_rel \<longleftrightarrow> aaa = {#}\<close> and
+  empty_list_mset_rel_iff:
+    \<open>(a, {#}) \<in> list_mset_rel \<longleftrightarrow> a = []\<close>
+  by (auto simp: list_mset_rel_def br_def)
+
+
+lemma snd_hnr_pure:
+   \<open>CONSTRAINT is_pure B \<Longrightarrow> (return \<circ> snd, RETURN \<circ> snd) \<in> A\<^sup>d *\<^sub>a B\<^sup>k \<rightarrow>\<^sub>a B\<close>
+  apply sepref_to_hoare
+  apply sep_auto
+  by (metis SLN_def SLN_left assn_times_comm ent_pure_pre_iff_sng ent_refl ent_star_mono
+      ent_true is_pure_assn_def is_pure_iff_pure_assn)
+
+text \<open>
+  This theorem is useful to debug situation where sepref is not able to synthesize a program (with
+  the ``[[unify\_trace\_failure]]'' to trace what fails in rule rule and the \<^text>\<open>to_hnr\<close> to
+  ensure the theorem has the correct form).
+\<close>
+lemma Pair_hnr: \<open>(uncurry (return oo (\<lambda>a b. Pair a b)), uncurry (RETURN oo (\<lambda>a b. Pair a b))) \<in>
+    A\<^sup>d *\<^sub>a B\<^sup>d \<rightarrow>\<^sub>a prod_assn A B\<close>
+  by sepref_to_hoare sep_auto
+
+
+text \<open>This version works only for \<^emph>\<open>pure\<close> refinement relations:\<close>
+lemma the_hnr_keep:
+  \<open>CONSTRAINT is_pure A \<Longrightarrow> (return o the, RETURN o the) \<in> [\<lambda>D. D \<noteq> None]\<^sub>a (option_assn A)\<^sup>k \<rightarrow> A\<close>
+  using pure_option[of A]
+  by sepref_to_hoare
+   (sep_auto simp: option_assn_alt_def is_pure_def split: option.splits)
+
+definition list_rel_mset_rel where list_rel_mset_rel_internal:
+\<open>list_rel_mset_rel \<equiv> \<lambda>R. \<langle>R\<rangle>list_rel O list_mset_rel\<close>
+
+lemma list_rel_mset_rel_def[refine_rel_defs]:
+  \<open>\<langle>R\<rangle>list_rel_mset_rel = \<langle>R\<rangle>list_rel O list_mset_rel\<close>
+  unfolding relAPP_def list_rel_mset_rel_internal ..
+
+lemma list_mset_assn_pure_conv:
+  \<open>list_mset_assn (pure R) = pure (\<langle>R\<rangle>list_rel_mset_rel)\<close>
+  apply (intro ext)
+  using list_all2_reorder_left_invariance
+  by (fastforce
+    simp: list_rel_mset_rel_def list_mset_assn_def
+      mset_rel_def rel2p_def[abs_def] rel_mset_def p2rel_def
+      list_mset_rel_def[abs_def] Collect_eq_comp br_def
+      list_rel_def Collect_eq_comp_right
+    intro!: arg_cong[of _ _ \<open>\<lambda>b. pure b _ _\<close>])
+
+lemma list_assn_list_mset_rel_eq_list_mset_assn:
+  assumes p: \<open>is_pure R\<close>
+  shows \<open>hr_comp (list_assn R) list_mset_rel = list_mset_assn R\<close>
+proof -
+  define R' where \<open>R' = the_pure R\<close>
+  then have R: \<open>R = pure R'\<close>
+    using p by auto
+  show ?thesis
+    apply (auto simp: list_mset_assn_def
+        list_assn_pure_conv
+        relcomp.simps hr_comp_pure mset_rel_def br_def
+        p2rel_def rel2p_def[abs_def] rel_mset_def R list_mset_rel_def list_rel_def)
+      using list_all2_reorder_left_invariance by fastforce
+  qed
+
+lemma list_rel_mset_rel_imp_same_length: \<open>(a, b) \<in> \<langle>R\<rangle>list_rel_mset_rel \<Longrightarrow> length a = size b\<close>
+  by (auto simp: list_rel_mset_rel_def list_mset_rel_def br_def
+      dest: list_rel_imp_same_length)
+
+
+lemma id_ref: \<open>(return o id, RETURN o id) \<in> R\<^sup>d \<rightarrow>\<^sub>a R\<close>
+  by sepref_to_hoare sep_auto
+
+text \<open>This functions deletes all elements of a resizable array, without resizing it.\<close>
+definition emptied_arl :: \<open>'a array_list \<Rightarrow> 'a array_list\<close> where
+\<open>emptied_arl = (\<lambda>(a, n). (a, 0))\<close>
+
+lemma emptied_arl_refine[sepref_fr_rules]:
+  \<open>(return o emptied_arl, RETURN o emptied_list) \<in> (arl_assn R)\<^sup>d \<rightarrow>\<^sub>a arl_assn R\<close>
+  unfolding emptied_arl_def emptied_list_def
+  by sepref_to_hoare (sep_auto simp: arl_assn_def hr_comp_def is_array_list_def)
+
+lemma bool_assn_alt_def: \<open>bool_assn a b = \<up> (a = b)\<close>
+  unfolding pure_def by auto
+
+lemma nempty_list_mset_rel_iff: \<open>M \<noteq> {#} \<Longrightarrow>
+  (xs, M) \<in> list_mset_rel \<longleftrightarrow> (xs \<noteq> [] \<and> hd xs \<in># M \<and>
+         (tl xs, remove1_mset (hd xs) M) \<in> list_mset_rel)\<close>
+  by (cases xs) (auto simp: list_mset_rel_def br_def dest!: multi_member_split)
+
+abbreviation ghost_assn where
+  \<open>ghost_assn \<equiv> hr_comp unit_assn virtual_copy_rel\<close>
+
+lemma [sepref_fr_rules]:
+ \<open>(return o (\<lambda>_. ()), RETURN o virtual_copy) \<in> R\<^sup>k \<rightarrow>\<^sub>a ghost_assn\<close>
+ by sepref_to_hoare (sep_auto simp: virtual_copy_rel_def)
+
+
+lemma id_mset_list_assn_list_mset_assn:
+  assumes \<open>CONSTRAINT is_pure R\<close>
+  shows \<open>(return o id, RETURN o mset) \<in> (list_assn R)\<^sup>d \<rightarrow>\<^sub>a list_mset_assn R\<close>
+proof -
+  obtain R' where R: \<open>R = pure R'\<close>
+    using assms is_pure_conv unfolding CONSTRAINT_def by blast
+  then have R': \<open>the_pure R = R'\<close>
+    unfolding R by auto
+  show ?thesis
+    apply (subst R)
+    apply (subst list_assn_pure_conv)
+    apply sepref_to_hoare
+    by (sep_auto simp: list_mset_assn_def R' pure_def list_mset_rel_def mset_rel_def
+       p2rel_def rel2p_def[abs_def] rel_mset_def br_def Collect_eq_comp list_rel_def)
+qed
+
+subsection \<open>Sorting\<close>
+
+text \<open>Remark that we do not \<^emph>\<open>prove\<close> that the sorting in correct, since we do not care about the
+ correctness, only the fact that it is reordered. (Based on wikipedia's algorithm.)
+Typically \<^term>\<open>R\<close> would be \<^term>\<open>(<)\<close>\<close>
+definition insert_sort_inner :: \<open>('b \<Rightarrow> 'b \<Rightarrow> bool) \<Rightarrow> ('a list \<Rightarrow> nat \<Rightarrow> 'b) \<Rightarrow> 'a list \<Rightarrow>  nat \<Rightarrow> 'a list nres\<close> where
+  \<open>insert_sort_inner R f xs i = do {
+     (j, ys) \<leftarrow> WHILE\<^sub>T\<^bsup>\<lambda>(j, ys). j \<ge> 0 \<and> mset xs = mset ys \<and> j < length ys\<^esup>
+         (\<lambda>(j, ys). j > 0 \<and> R (f ys j) (f ys (j - 1)))
+         (\<lambda>(j, ys). do {
+             ASSERT(j < length ys);
+             ASSERT(j > 0);
+             ASSERT(j-1 < length ys);
+             let xs = swap ys j (j - 1);
+             RETURN (j-1, xs)
+           }
+         )
+        (i, xs);
+     RETURN ys
+  }\<close>
+
+
+(* A check: *)
+lemma \<open>RETURN [Suc 0, 2, 0] = insert_sort_inner (<) (\<lambda>remove n. remove ! n) [2::nat, 1, 0] 1\<close>
+  by (simp add: WHILEIT_unfold insert_sort_inner_def swap_def)
+
+definition reorder_remove :: \<open>'b \<Rightarrow> 'a list \<Rightarrow> 'a list nres\<close> where
+\<open>reorder_remove _ removed = SPEC (\<lambda>removed'. mset removed' = mset removed)\<close>
+
+definition insert_sort :: \<open>('b \<Rightarrow> 'b \<Rightarrow> bool) \<Rightarrow> ('a list \<Rightarrow> nat \<Rightarrow> 'b) \<Rightarrow> 'a list \<Rightarrow> 'a list nres\<close> where
+  \<open>insert_sort R f xs = do {
+     (i, ys) \<leftarrow> WHILE\<^sub>T\<^bsup>\<lambda>(i, ys). (ys = [] \<or> i \<le> length ys) \<and> mset xs = mset ys\<^esup>
+        (\<lambda>(i, ys). i < length ys)
+        (\<lambda>(i, ys). do {
+            ASSERT(i < length ys);
+            ys \<leftarrow> insert_sort_inner R f ys i;
+            RETURN (i+1, ys)
+          })
+        (1, xs);
+     RETURN ys
+  }\<close>
+
+lemma insert_sort_inner:
+   \<open>(uncurry (insert_sort_inner R f), uncurry (\<lambda>m m'. reorder_remove m' m)) \<in>
+      [\<lambda>(xs, i). i < length xs]\<^sub>f \<langle>Id:: ('a \<times> 'a) set\<rangle>list_rel \<times>\<^sub>r nat_rel \<rightarrow> \<langle>Id\<rangle> nres_rel\<close>
+  unfolding insert_sort_inner_def uncurry_def reorder_remove_def
+  apply (intro frefI nres_relI)
+  apply clarify
+  apply (refine_vcg WHILEIT_rule[where R = \<open>measure (\<lambda>(i, _). i)\<close>])
+  subgoal by auto
+  subgoal by auto
+  subgoal by auto
+  subgoal by auto
+  subgoal by (auto dest: mset_eq_length)
+  subgoal by auto
+  subgoal by auto
+  subgoal by auto
+  subgoal by auto
+  subgoal by auto
+  subgoal by auto
+  subgoal by auto
+  done
+
+lemma insert_sort_reorder_remove:
+  \<open>(insert_sort R f, reorder_remove vm) \<in> \<langle>Id\<rangle>list_rel \<rightarrow>\<^sub>f \<langle>Id\<rangle> nres_rel\<close>
+proof -
+  have H: \<open>ba < length aa \<Longrightarrow> insert_sort_inner R f aa ba \<le> SPEC (\<lambda>m'. mset m' = mset aa)\<close>
+    for ba aa
+    using insert_sort_inner[unfolded fref_def nres_rel_def reorder_remove_def, simplified]
+    by fast
+  show ?thesis
+    unfolding insert_sort_def reorder_remove_def
+    apply (intro frefI nres_relI)
+    apply (refine_vcg WHILEIT_rule[where R = \<open>measure (\<lambda>(i, ys). length ys - i)\<close>] H)
+    subgoal by auto
+    subgoal by auto
+    subgoal by auto
+    subgoal by auto
+    subgoal by (auto dest: mset_eq_length)
+    subgoal by auto
+    subgoal by (auto dest!: mset_eq_length)
+    subgoal by auto
+    done
+qed
+
+definition arl_replicate where
+ "arl_replicate init_cap x \<equiv> do {
+    let n = max init_cap minimum_capacity;
+    a \<leftarrow> Array.new n x;
+    return (a,init_cap)
+  }"
+
+definition \<open>op_arl_replicate = op_list_replicate\<close>
+lemma arl_fold_custom_replicate:
+  \<open>replicate = op_arl_replicate\<close>
+  unfolding op_arl_replicate_def op_list_replicate_def ..
+
+lemma list_replicate_arl_hnr[sepref_fr_rules]:
+  assumes p: \<open>CONSTRAINT is_pure R\<close>
+  shows \<open>(uncurry arl_replicate, uncurry (RETURN oo op_arl_replicate)) \<in> nat_assn\<^sup>k *\<^sub>a R\<^sup>k \<rightarrow>\<^sub>a arl_assn R\<close>
+proof -
+  obtain R' where
+     R'[symmetric]: \<open>R' = the_pure R\<close> and
+     R_R': \<open>R = pure R'\<close>
+    using assms by fastforce
+  have [simp]: \<open>pure R' b bi = \<up>((bi, b) \<in> R')\<close> for b bi
+    by (auto simp: pure_def)
+  have [simp]: \<open>min a (max a 16) = a\<close> for a :: nat
+    by auto
+  show ?thesis
+    using assms unfolding op_arl_replicate_def
+    by sepref_to_hoare
+      (sep_auto simp: arl_replicate_def arl_assn_def hr_comp_def R' R_R' list_rel_def
+        is_array_list_def minimum_capacity_def
+        intro!: list_all2_replicate)
+qed
+
+lemma option_bool_assn_direct_eq_hnr:
+  \<open>(uncurry (return oo (=)), uncurry (RETURN oo (=))) \<in>
+    (option_assn bool_assn)\<^sup>k *\<^sub>a (option_assn bool_assn)\<^sup>k \<rightarrow>\<^sub>a bool_assn\<close>
+  by sepref_to_hoare (sep_auto simp: option_assn_alt_def split:option.splits)
+
+text \<open>This function does not change the size of the underlying array.\<close>
+definition take1 where
+  \<open>take1 xs = take 1 xs\<close>
+
+lemma take1_hnr[sepref_fr_rules]:
+  \<open>(return o (\<lambda>(a, _). (a, 1::nat)), RETURN o take1) \<in> [\<lambda>xs. xs \<noteq> []]\<^sub>a (arl_assn R)\<^sup>d \<rightarrow> arl_assn R\<close>
+  apply sepref_to_hoare
+  apply (sep_auto simp: arl_assn_def hr_comp_def take1_def list_rel_def
+      is_array_list_def)
+  apply (case_tac b; case_tac x; case_tac l')
+   apply (auto)
+  done
+
+text \<open>The following two abbreviation are variants from \<^term>\<open>uncurry4\<close> and
+   \<^term>\<open>uncurry6\<close>. The problem is that \<^term>\<open>uncurry2 (uncurry2 f)\<close> and
+   \<^term>\<open>uncurry (uncurry3 f)\<close> are the same term, but only the latter is folded
+   to \<^term>\<open>uncurry4\<close>.\<close>
+abbreviation uncurry4' where
+  "uncurry4' f \<equiv> uncurry2 (uncurry2 f)"
+
+abbreviation uncurry6' where
+  "uncurry6' f \<equiv> uncurry2 (uncurry4' f)"
+
+
+definition find_in_list_between :: \<open>('a \<Rightarrow> bool) \<Rightarrow> nat \<Rightarrow> nat \<Rightarrow> 'a list \<Rightarrow> nat option nres\<close> where
+  \<open>find_in_list_between P a b C = do {
+      (x, _) \<leftarrow> WHILE\<^sub>T\<^bsup>\<lambda>(found, i). i \<ge> a \<and> i \<le> length C \<and> i \<le> b \<and> (\<forall>j\<in>{a..<i}. \<not>P (C!j)) \<and>
+        (\<forall>j. found = Some j \<longrightarrow> (i = j \<and> P (C ! j) \<and> j < b \<and> j \<ge> a))\<^esup>
+        (\<lambda>(found, i). found = None \<and> i < b)
+        (\<lambda>(_, i). do {
+          ASSERT(i < length C);
+          if P (C!i) then RETURN (Some i, i) else RETURN (None, i+1)
+        })
+        (None, a);
+      RETURN x
+  }\<close>
+
+lemma find_in_list_between_spec:
+  assumes \<open>a \<le> length C\<close> and \<open>b \<le> length C\<close> and \<open>a \<le> b\<close>
+  shows
+    \<open>find_in_list_between P a b C \<le> SPEC(\<lambda>i.
+       (i \<noteq> None \<longrightarrow>  P (C ! the i) \<and> the i \<ge> a \<and> the i < b) \<and>
+       (i = None \<longrightarrow> (\<forall>j. j \<ge> a \<longrightarrow> j < b \<longrightarrow> \<not>P (C!j))))\<close>
+  unfolding find_in_list_between_def
+  apply (refine_vcg WHILEIT_rule[where R = \<open>measure (\<lambda>(f, i). Suc (length C) - (i + (if f = None then 0 else 1)))\<close>])
+  subgoal by auto
+  subgoal by auto
+  subgoal using assms by auto
+  subgoal using assms by auto
+  subgoal by auto
+  subgoal by auto
+  subgoal by auto
+  subgoal by auto
+  subgoal by auto
+  subgoal using assms by auto
+  subgoal by auto
+  subgoal by auto
+  subgoal by auto
+  subgoal by auto
+  subgoal by auto
+  subgoal by auto
+  subgoal by auto
+  subgoal by auto
+  subgoal by auto
+  subgoal by auto
+  subgoal by auto
+  subgoal by auto
+  subgoal by (auto simp: less_Suc_eq)
+  subgoal by auto
+  subgoal by auto
+  subgoal by auto
+  subgoal by auto
+  subgoal by auto
+  subgoal by auto
+  subgoal by auto
+  subgoal by auto
+  subgoal by auto
+  done
+
+lemma list_assn_map_list_assn: \<open>list_assn g (map f x) xi = list_assn (\<lambda>a c. g (f a) c) x xi\<close>
+  apply (induction x arbitrary: xi)
+  subgoal by auto
+  subgoal for a x xi
+    by (cases xi) auto
+  done
+
+end
